compiler/bootstrap/compilation/arm8/64/arm8SexprBootstrap64Script.sml
@@ -1,0 +1,14 @@
+(*
+  S-expression release artifact for the native ARM8 compiler.
+*)
+Theory arm8SexprBootstrap64
+Ancestors
+  compiler64Arm8Prog
+Libs
+  preamble mlstringSyntax astSyntax astToSexprLib
+
+val _ = compiler64_arm8_prog_def
+          |> CONV_RULE (RAND_CONV EVAL)
+          |> concl
+          |> rhs
+          |> write_ast_to_file "cake-sexpr-64";
