compiler/bootstrap/compilation/arm8/64/proofs/arm8BootstrapProofScript.sml
@@ -3,8 +3,10 @@
 *)
 Theory arm8BootstrapProof
 Ancestors
-  repl_decs_allowed semanticsProps backendProof arm8_configProof
-  compiler64Prog arm8Bootstrap
+  holLightConsistency
+  semanticsProps backendProof arm8_configProof arm8_asl_configProof
+  compiler64Arm8Prog arm8Bootstrap arm8ReplProof compiler64ReplProof
+  candle_prover_semantics mlstring
 Libs
   preamble
 
@@ -38,8 +40,22 @@ Proof
   fs [compiler_instance_def]
 QED
 
+Theorem backend_config_ok_init_conf:
+  backend_config_ok arm8_config init_conf
+Proof
+  assume_tac arm8_backend_config_ok
+  \\ gvs [backendProofTheory.backend_config_ok_def,init_conf_def]
+  \\ EVAL_TAC
+QED
+
+Theorem mc_init_ok_init_conf:
+  mc_init_ok arm8_config init_conf mc = mc_init_ok arm8_config arm8_backend_config mc
+Proof
+  simp [mc_init_ok_def,init_conf_def]
+QED
+
 val cake_io_events_def = new_specification("cake_io_events_def",["cake_io_events"],
-  semantics_compiler64_prog
+  semantics_compiler64_arm8_prog
   |> SRULE [ml_progTheory.prog_syntax_ok_semantics, compiler64_compiled]
   |> Q.INST[‘eval_state_var’|->‘the_EvalDecs (mk_init_eval_state compiler_instance)’]
   |> SIMP_RULE (srw_ss()) [source_evalProofTheory.mk_init_eval_state_def,the_EvalDecs_def]
@@ -57,9 +73,9 @@ val compile_correct_applied =
                          GSYM AND_IMP_INTRO,with_clos_conf_simp]
   |> Q.INST [‘ev’|->‘SOME compiler_instance’]
   |> SIMP_RULE (srw_ss()) [add_eval_state_def,opt_eval_config_wf_def,
-                           compiler_instance_lemma]
+                           compiler_instance_lemma,mc_init_ok_init_conf]
   |> C MATCH_MP cake_not_fail
-  |> C MATCH_MP arm8_backend_config_ok
+  |> C MATCH_MP backend_config_ok_init_conf
   |> REWRITE_RULE[cake_sem_sing,AND_IMP_INTRO]
   |> REWRITE_RULE[Once (GSYM AND_IMP_INTRO)]
   |> C MATCH_MP (CONJ(UNDISCH arm8_machine_config_ok)(UNDISCH arm8_init_ok))
@@ -69,4 +85,273 @@ val compile_correct_applied =
 Theorem cake_compiled_thm =
   CONJ compile_correct_applied cake_output
   |> DISCH_ALL
-  |> check_thm;
+
+val compile_correct_applied_asl =
+  MATCH_MP compile_correct_eval (cj 1 compiler64_compiled)
+  |> SIMP_RULE(srw_ss())[LET_THM,ml_progTheory.init_state_env_thm,
+                         GSYM AND_IMP_INTRO,with_clos_conf_simp]
+  |> Q.INST [‘ev’|->‘SOME compiler_instance’]
+  |> SIMP_RULE (srw_ss()) [add_eval_state_def,opt_eval_config_wf_def,
+                           compiler_instance_lemma,mc_init_ok_init_conf]
+  |> C MATCH_MP cake_not_fail
+  |> C MATCH_MP backend_config_ok_init_conf
+  |> REWRITE_RULE[cake_sem_sing,AND_IMP_INTRO]
+  |> REWRITE_RULE[Once (GSYM AND_IMP_INTRO)]
+  |> C MATCH_MP (CONJ(UNDISCH arm8_asl_machine_config_ok)
+                     (UNDISCH arm8_asl_init_ok))
+  |> DISCH(#1(dest_imp(concl arm8_asl_init_ok)))
+  |> REWRITE_RULE[AND_IMP_INTRO]
+
+Theorem cake_compiled_asl_thm =
+  CONJ compile_correct_applied_asl cake_output
+  |> DISCH_ALL
+
+(* --- *)
+
+Theorem mk_compiler_fun_from_ci_tuple[local]:
+  mk_compiler_fun_from_ci c = (λ(x,y,z). mk_compiler_fun_from_ci c (x,y,z))
+Proof
+  fs [FUN_EQ_THM,FORALL_PROD]
+QED
+
+Theorem mk_init_eval_state_lemma =
+  “mk_init_eval_state compiler_instance”
+  |> SIMP_CONV (srw_ss()) [compiler_instance_def,
+       source_evalProofTheory.mk_init_eval_state_def]
+  |> ONCE_REWRITE_RULE [mk_compiler_fun_from_ci_tuple]
+  |> SIMP_RULE (srw_ss()) [source_evalProofTheory.mk_compiler_fun_from_ci_def,
+        GSYM compiler64ReplProofTheory.compiler_inst_def];
+
+Overload init_eval_state_for =
+  “λext cl fs. (init_state (basis_ffi ext cl fs) with
+        eval_state := SOME (mk_init_eval_state compiler_instance))”
+
+Theorem candle_soundness:
+  res ∈ semantics_prog (init_eval_state_for ext cl fs) init_env (candle_code ++ prog) ∧
+  EVERY safe_dec prog ∧ prog_syntax_ok candle_code ∧ res ≠ Fail
+  ⇒
+  ∀e. e ∈ events_of res ⇒ ok_event e
+Proof
+  rw [IN_DEF]
+  \\ drule_then irule events_of_semantics_with_eval_state
+  \\ fs [IN_DEF]
+  \\ simp [basis_ffiTheory.basis_ffi_def]
+  \\ fs [candle_prover_invTheory.eval_state_ok_def,mk_init_eval_state_lemma]
+  \\ fs [source_evalProofTheory.v_rel_abs]
+  \\ rpt gen_tac
+  \\ DEEP_INTRO_TAC some_intro
+  \\ fs [repl_decs_allowedTheory.decs_allowed_def,IN_DEF]
+QED
+
+Theorem repl_not_fail =
+  semantics_prog_compiler64_arm8_prog
+  |> Q.GEN ‘s’ |> ISPEC (mk_init_eval_state_lemma |> concl |> rand |> rand)
+  |> REWRITE_RULE [GSYM mk_init_eval_state_lemma]
+  |> SIMP_RULE (srw_ss()) [IN_DEF]
+  |> Q.GEN ‘conf’ |> Q.SPEC ‘info’
+  |> REWRITE_RULE [GSYM (SIMP_CONV (srw_ss()) [] “hasFreeFD fs”)];
+
+Overload basis_init_ok =
+  “λcl fs. STD_streams fs ∧ wfFS fs ∧ wfcl cl ∧ hasFreeFD fs ∧
+           file_content fs «config_enc_str.txt» = SOME conf”;
+
+Theorem repl_not_fail_thm:
+  has_repl_flag (TL cl) ∧ basis_init_ok cl fs ⇒
+  Fail ∉ semantics_prog (init_eval_state_for ext cl fs) init_env compiler64_arm8_prog
+Proof
+  rw [IN_DEF] \\ irule repl_not_fail \\ fs []
+  \\ simp [compiler64_compiled]
+QED
+
+val compile_correct_applied2 =
+  MATCH_MP compile_correct_eval (cj 1 compiler64_compiled)
+  |> SIMP_RULE(srw_ss())[LET_THM,ml_progTheory.init_state_env_thm,
+                         GSYM AND_IMP_INTRO,with_clos_conf_simp]
+  |> Q.INST [‘ev’|->‘SOME compiler_instance’]
+  |> SIMP_RULE (srw_ss()) [add_eval_state_def,opt_eval_config_wf_def,
+      arm8_configProofTheory.arm8_backend_config_ok,compiler_instance_lemma]
+  |> Q.GEN ‘ffi’ |> Q.ISPEC ‘basis_ffi ext cl fs’
+
+Definition repl_ready_to_run_def:
+  repl_ready_to_run cl fs (mc,ms) ⇔
+    ∃cbspace data_sp.
+      has_repl_flag (TL cl) ∧ wfcl cl ∧ wfFS fs ∧ STD_streams fs ∧
+      hasFreeFD fs ∧
+      file_content fs «config_enc_str.txt» = SOME conf ∧
+      is_arm8_asl_machine_config mc ∧
+      installed code cbspace data data_sp
+        info.lab_conf.ffi_names
+        (heap_regs arm8_backend_config.stack_conf.reg_names)
+        mc info.lab_conf.shmem_extra ms
+End
+
+Overload machine_sem = “λffi (mc,ms). targetSem$machine_sem mc ffi ms”
+
+Theorem compile_correct_applied:
+  Fail ∉ semantics_prog (init_eval_state_for ext cl fs) init_env compiler64_arm8_prog ∧
+  repl_ready_to_run cl fs ms ⇒
+  machine_sem (basis_ffi ext cl fs) ms ⊆
+    extend_with_resource_limit
+      (semantics_prog (init_eval_state_for ext cl fs) init_env compiler64_arm8_prog)
+Proof
+  PairCases_on ‘ms’ \\ rw [IN_DEF,repl_ready_to_run_def]
+  \\ irule compile_correct_applied2 \\ fs []
+  \\ ‘init_conf.stack_conf.reg_names =
+      arm8_backend_config.stack_conf.reg_names’ by EVAL_TAC
+  \\ gvs [] \\ first_x_assum $ irule_at Any
+  \\ gvs [backend_config_ok_init_conf,mc_init_ok_init_conf,
+          arm8_asl_machine_config_ok,arm8_asl_init_ok]
+QED
+
+Theorem isPREFIX_MEM[local]:
+  ∀xs ys. isPREFIX xs ys ⇒ ∀x. MEM x xs ⇒ MEM x ys
+Proof
+  Induct \\ fs [] \\ Cases_on ‘ys’ \\ fs [] \\ metis_tac []
+QED
+
+Theorem LPREFIX_MEM[local]:
+  ∀xs ys. LPREFIX (fromList xs) ys ⇒ ∀x. MEM x xs ⇒ x IN LSET ys
+Proof
+  Induct \\ fs [] \\ Cases_on ‘ys’ \\ fs []
+  \\ fs [LPREFIX_LCONS] \\ metis_tac []
+QED
+
+Theorem repl_ready_to_run_imp:
+  repl_ready_to_run cl fs ms ⇒
+  has_repl_flag (TL cl) ∧ basis_init_ok cl fs
+Proof
+  PairCases_on ‘ms’ \\ rw [repl_ready_to_run_def] \\ fs []
+QED
+
+Theorem prog_syntax_ok_candle_code[local]:
+  prog_syntax_ok candle_code
+Proof
+  ‘prog_syntax_ok compiler64_arm8_prog’ by fs [compiler64_compiled]
+  \\ irule ml_progTheory.prog_syntax_ok_isPREFIX
+  \\ first_x_assum $ irule_at Any
+  \\ strip_assume_tac compiler64_arm8_prog_eq_candle_code_append
+  \\ gvs []
+QED
+
+Theorem events_of_extend_with_resource_limit:
+  e ∈ events_of res1 ∧ res1 ∈ sem1 ∧
+  sem1 ⊆ extend_with_resource_limit sem2 ⇒
+  ∃res2. e ∈ events_of res2 ∧ res2 ∈ sem2
+Proof
+  fs [IN_DEF,SUBSET_DEF,extend_with_resource_limit_def] \\ rw []
+  \\ first_x_assum drule \\ fs [] \\ rw []
+  \\ first_assum $ irule_at Any \\ fs [events_of_def]
+  \\ imp_res_tac isPREFIX_MEM \\ fs [IN_DEF]
+  \\ imp_res_tac LPREFIX_MEM \\ fs [IN_DEF]
+QED
+
+Theorem candle_top_level_soundness:
+  repl_ready_to_run cl fs ms ∧ res ∈ machine_sem (basis_ffi ext cl fs) ms ⇒
+  res ≠ Fail ∧
+  ∀e. e ∈ events_of res ⇒ ok_event e
+Proof
+  strip_tac
+  \\ drule_all_then strip_assume_tac repl_ready_to_run_imp
+  \\ imp_res_tac repl_not_fail_thm
+  \\ first_x_assum $ qspec_then ‘ext’ assume_tac
+  \\ drule_all compile_correct_applied
+  \\ strip_tac
+  \\ ‘res ≠ Fail’ by
+   (CCONTR_TAC \\ gvs [IN_DEF,extend_with_resource_limit_def,SUBSET_DEF]
+    \\ first_x_assum drule \\ fs [])
+  \\ rw []
+  \\ drule_all events_of_extend_with_resource_limit \\ rw []
+  \\ strip_assume_tac compiler64_arm8_prog_eq_candle_code_append \\ gvs []
+  \\ drule_then irule candle_soundness
+  \\ fs [prog_syntax_ok_candle_code] \\ CCONTR_TAC \\ fs []
+QED
+
+(* Every byte string the kernel writes on its own channel decodes back to the
+   theorem and the context it was proved in, and that context extends the
+   initial one. So a reader of the channel can decide the shape of the context
+   and, when it is one of the shapes a HOL Light session builds, conclude that
+   the theory the theorem lives in is consistent. *)
+
+Theorem candle_top_level_consistency_axiom_free:
+  repl_ready_to_run cl fs ms ∧ res ∈ machine_sem (basis_ffi ext cl fs) ms ⇒
+  res ≠ Fail ∧
+  ∀out y. IO_event (ExtCall kernel_ffi) out y ∈ events_of res ⇒
+    ∃ctxt th.
+      THM ctxt th ∧ thm2bytes ctxt th = out ∧
+      string_to_thm (bytes2str out) = (ctxt,th) ∧
+      ctxt extends init_ctxt ∧
+      (axiom_free ctxt ⇒ consistent_theory (thyof ctxt))
+Proof
+  strip_tac
+  \\ drule_all candle_top_level_soundness
+  \\ strip_tac \\ simp []
+  \\ rpt strip_tac
+  \\ first_x_assum drule
+  \\ simp [candle_kernel_valsTheory.ok_event_def]
+  \\ strip_tac
+  \\ first_assum $ irule_at Any
+  \\ gvs [candle_kernel_valsTheory.bytes2str_thm2bytes,
+          print_thmTheory.string_to_thm_thm_to_string]
+  \\ strip_tac
+  \\ irule init_light_consistent \\ gs []
+QED
+
+Theorem candle_top_level_consistency_fhol_light:
+  repl_ready_to_run cl fs ms ∧ res ∈ machine_sem (basis_ffi ext cl fs) ms ⇒
+  res ≠ Fail ∧
+  ∀out y. IO_event (ExtCall kernel_ffi) out y ∈ events_of res ⇒
+    ∃ctxt th.
+      THM ctxt th ∧ thm2bytes ctxt th = out ∧
+      string_to_thm (bytes2str out) = (ctxt,th) ∧
+      ctxt extends init_ctxt ∧
+      (fhol_light_ctxt ctxt ⇒ consistent_theory (thyof ctxt))
+Proof
+  strip_tac
+  \\ drule_all candle_top_level_soundness
+  \\ strip_tac \\ simp []
+  \\ rpt strip_tac
+  \\ first_x_assum drule
+  \\ simp [candle_kernel_valsTheory.ok_event_def]
+  \\ strip_tac
+  \\ first_assum $ irule_at Any
+  \\ gvs [candle_kernel_valsTheory.bytes2str_thm2bytes,
+          print_thmTheory.string_to_thm_thm_to_string]
+  \\ strip_tac
+  \\ irule fhol_light_consistent \\ gs []
+QED
+
+Theorem candle_top_level_consistency_hol_light:
+  repl_ready_to_run cl fs ms ∧ res ∈ machine_sem (basis_ffi ext cl fs) ms ⇒
+  res ≠ Fail ∧
+  ∀out y. IO_event (ExtCall kernel_ffi) out y ∈ events_of res ⇒
+    ∃ctxt th.
+      THM ctxt th ∧ thm2bytes ctxt th = out ∧
+      string_to_thm (bytes2str out) = (ctxt,th) ∧
+      ctxt extends init_ctxt ∧
+      (hol_light_ctxt ctxt ∧ (∃inf. is_infinite V_mem inf) ⇒
+         consistent_theory (thyof ctxt))
+Proof
+  strip_tac
+  \\ drule_all candle_top_level_soundness
+  \\ strip_tac \\ simp []
+  \\ rpt strip_tac
+  \\ first_x_assum drule
+  \\ simp [candle_kernel_valsTheory.ok_event_def]
+  \\ strip_tac
+  \\ first_assum $ irule_at Any
+  \\ gvs [candle_kernel_valsTheory.bytes2str_thm2bytes,
+          print_thmTheory.string_to_thm_thm_to_string]
+  (* keep the existential intact: hol_light_consistent's hypothesis is where
+     the set-theory universe type gets fixed, and the conclusion does not
+     mention it *)
+  \\ disch_then (CONJUNCTS_THEN assume_tac)
+  \\ drule_then irule hol_light_consistent \\ gs []
+QED
+
+val _ = print "Checking that no cheats were used in the proofs.\n";
+val _ = candle_top_level_soundness |> check_thm;
+val _ = candle_top_level_consistency_axiom_free |> check_thm;
+val _ = candle_top_level_consistency_fhol_light |> check_thm;
+val _ = candle_top_level_consistency_hol_light |> check_thm;
+val _ = cake_compiled_thm |> check_thm;
+val _ = cake_compiled_asl_thm |> check_thm;
