compiler/bootstrap/compilation/arm8/64/proofs/arm8ReplProofScript.sml
@@ -1,16 +1,22 @@
 (*
-  Verification of the function (called repl) that implements the REPL
+  Source-level REPL and Candle properties of the native ARM8 compiler.
 *)
-Theory replProof
+Theory arm8ReplProof
 Ancestors
-  semanticsProps backendProof x64_configProof compiler64Prog
+  semanticsProps backendProof arm8_configProof compiler64Arm8Prog
   compiler64MainProg compiler64Host compiler64ReplProof
   evaluate semanticPrimitives ml_translator repl_types
-  repl_check_and_tweak repl_init
+  repl_check_and_tweak repl_init candle_prover_inv
 Libs
-  preamble
+  preamble ml_progLib
 
-val _ = (max_print_depth := 12);
+Theorem repl_prog_isPREFIX:
+  repl_prog ≼ FRONT compiler64_arm8_prog
+Proof
+  rewrite_tac [listTheory.isPREFIX_THM,repl_moduleProgTheory.repl_prog_def,
+               compiler64Arm8ProgTheory.compiler64_arm8_prog_def,FRONT_CONS,
+               locationTheory.unknown_loc_def]
+QED
 
 Theorem BACKEND_CONFIG_TYPE_v[local]:
   BACKEND_CONFIG_TYPE conf u ⇒
@@ -19,65 +25,52 @@ Proof
   rw [] \\ imp_res_tac BACKEND_CONFIG_IMP \\ fs []
 QED
 
-Theorem repl_prog_isPREFIX:
-  repl_prog ≼ FRONT compiler64_prog
-Proof
-  rewrite_tac [listTheory.isPREFIX_THM,repl_moduleProgTheory.repl_prog_def,
-               compiler64ProgTheory.compiler64_prog_def,FRONT_CONS,
-               locationTheory.unknown_loc_def]
-  \\ EVAL_TAC
-QED
-
 val ffi_inst = type_of “basis_ffi _ _ _” |> dest_type |> snd |> hd
 
-(*
-  max_print_depth := 15
-*)
-
-Theorem evaluate_decs_compiler64_prog:
-  s.compiler = compiler_inst x64_config ∧
+Theorem evaluate_decs_compiler64_arm8_prog:
+  s.compiler = compiler_inst arm8_config ∧
   s.decode_decs = v_fun_abs decs_allowed (LIST_v DEC_v) ∧
-  s.env_id_counter = (0,0,1) ∧ prog_syntax_ok compiler64_prog ∧
+  s.env_id_counter = (0,0,1) ∧ prog_syntax_ok compiler64_arm8_prog ∧
   has_repl_flag (TL cl) ∧ wfcl cl ∧ wfFS fs ∧ STD_streams fs ∧ hasFreeFD fs ∧
   s.compiler_state = BACKEND_CONFIG_v conf ∧
   file_content fs «config_enc_str.txt» = SOME (encode_backend_config conf) ∧
   evaluate_decs (init_state (basis_ffi ext cl fs) with
                             <| clock := ck; eval_state := (SOME (EvalDecs s)) |>)
-      init_env compiler64_prog = (s1,res) ⇒
+      init_env compiler64_arm8_prog = (s1,res) ⇒
   res ≠ Rerr (Rabort Rtype_error)
 Proof
   rw [] \\ pop_assum mp_tac
-  \\ ‘~NULL compiler64_prog’ by
-   (once_rewrite_tac [compiler64_prog_def] \\ rewrite_tac [NULL])
+  \\ ‘~NULL compiler64_arm8_prog’ by (
+    once_rewrite_tac [compiler64_arm8_prog_def] \\ rewrite_tac [NULL])
   \\ drule BUTLAST_LAST
   \\ disch_then (once_rewrite_tac o single)
   \\ strip_tac
-  \\ assume_tac (Decls_FRONT_compiler64_prog
+  \\ assume_tac (Decls_FRONT_compiler64_arm8_prog
        |> REWRITE_RULE [ml_progTheory.ML_code_env_def]
        |> Q.GEN ‘ffi’ |> Q.ISPEC ‘basis_ffi ext cl fs’
        |> Q.INST [‘eval_state_var’|->‘s’])
   \\ dxrule ml_progTheory.Decls_IMP_Prog
-  \\ ‘prog_syntax_ok (FRONT compiler64_prog)’ by
-    (irule ml_progTheory.prog_syntax_ok_isPREFIX
-     \\ first_x_assum $ irule_at Any
-     \\ Cases_on ‘compiler64_prog’ using SNOC_CASES
-     \\ gvs [])
-  \\ ‘prog_syntax_ok repl_prog’ by
-    (irule ml_progTheory.prog_syntax_ok_isPREFIX
-     \\ irule_at Any repl_prog_isPREFIX \\ fs [])
+  \\ ‘prog_syntax_ok (FRONT compiler64_arm8_prog)’ by (
+    irule ml_progTheory.prog_syntax_ok_isPREFIX
+    \\ first_x_assum $ irule_at Any
+    \\ Cases_on ‘compiler64_arm8_prog’ using SNOC_CASES
+    \\ gvs [])
+  \\ ‘prog_syntax_ok repl_prog’ by (
+    irule ml_progTheory.prog_syntax_ok_isPREFIX
+    \\ irule_at Any repl_prog_isPREFIX \\ fs [])
   \\ impl_tac >- fs [] \\ strip_tac
   \\ drule (repl_types_repl_prog |> Q.INST [`entry_cost` |-> `3`])
   \\ disch_then drule
   \\ disch_then (qspec_then ‘encode_backend_config conf’ mp_tac)
-  \\ impl_tac >-
-   (fs [] \\ simp (DB.find "repl_moduleProg_st" |> map (#1 o #2))
+  \\ impl_tac >- (
+    fs [] \\ simp (DB.find "repl_moduleProg_st" |> map (#1 o #2))
     \\ simp (repl_prog_isPREFIX :: (DB.find "refs_def" |> map (#1 o #2)))
     \\ fs [repl_prog_st_def, ml_progTheory.init_state_def])
   \\ fs [repl_prog_st_def]
   \\ qpat_abbrev_tac ‘ppp = W8array _ :: _’ \\ pop_assum kall_tac
   \\ qpat_x_assum ‘Prog _ _ _ _ _’ kall_tac
   \\ qpat_x_assum ‘evaluate_decs _ _ _ = _’ kall_tac
-  \\ strip_tac \\ fs [LAST_compiler64_prog]
+  \\ strip_tac \\ fs [LAST_compiler64_arm8_prog]
   \\ qpat_x_assum ‘evaluate_decs _ _ _ = _’ mp_tac
   (* calling main *)
   \\ fs [evaluate_decs_def,astTheory.pat_bindings_def,
@@ -203,8 +196,8 @@ Proof
   \\ qspecl_then
        [‘st8’,‘env8’,‘Short «start_repl»’,‘Short « v0»’,‘basis_ffi ext cl fs’,‘TL cl’] mp_tac
     (evaluate_start_repl
-     |> Q.INST [`host` |-> `HostX64`,
-                `host_v` |-> `COMPILER64HOST_COMPILER64_HOST_v HostX64`]
+     |> Q.INST [`host` |-> `HostArm8`,
+                `host_v` |-> `COMPILER64HOST_COMPILER64_HOST_v HostArm8`]
      |> Q.GENL [`st`,`env`,`start_repl_str`,`arg_str`,`ffi`,`cl`,`s1`,`s`])
   \\ simp [Abbr`st8`,Abbr`env8`,Abbr`ev`,host_config_def,
            COMPILER64HOST_COMPILER64_HOST_TYPE_def,
@@ -215,8 +208,8 @@ Proof
   \\ disch_then drule
   \\ gvs []
   \\ impl_tac
-  >-
-   (CONV_TAC (DEPTH_CONV ml_progLib.nsLookup_conv) \\ simp [dec_clock_def]
+  >- (
+    CONV_TAC (DEPTH_CONV ml_progLib.nsLookup_conv) \\ simp [dec_clock_def]
     \\ irule repl_types_clock_refs
     \\ qsuff_tac ‘(s_pr with eval_state := NONE) = s_pr’ >- fs []
     \\ fs [semanticPrimitivesTheory.state_component_equality])
@@ -228,20 +221,128 @@ Proof
   \\ simp [pmatch_def] \\ rw [combine_dec_result_def] \\ fs []
 QED
 
-Theorem semantics_prog_compiler64_prog:
-  s.compiler = compiler_inst x64_config ∧
+Theorem semantics_prog_compiler64_arm8_prog:
+  s.compiler = compiler_inst arm8_config ∧
   s.decode_decs = v_fun_abs decs_allowed (LIST_v DEC_v) ∧
   s.env_id_counter = (0,0,1) ∧ has_repl_flag (TL cl) ∧ wfcl cl ∧ wfFS fs ∧
-  STD_streams fs ∧ hasFreeFD fs ∧ prog_syntax_ok compiler64_prog ∧
+  STD_streams fs ∧ hasFreeFD fs ∧ prog_syntax_ok compiler64_arm8_prog ∧
   s.compiler_state = BACKEND_CONFIG_v conf ∧
   file_content fs «config_enc_str.txt» = SOME (encode_backend_config conf) ⇒
   Fail ∉ semantics_prog
            (init_state (basis_ffi ext cl fs) with eval_state := SOME (EvalDecs s))
-           init_env compiler64_prog
+           init_env compiler64_arm8_prog
 Proof
   fs [IN_DEF,semanticsTheory.semantics_prog_def] \\ rpt strip_tac
-  \\ mp_tac (Q.GENL [‘ck’,‘res’,‘s1’] evaluate_decs_compiler64_prog) \\ fs []
+  \\ mp_tac (Q.GENL [‘ck’,‘res’,‘s1’] evaluate_decs_compiler64_arm8_prog) \\ fs []
   \\ fs [semanticsTheory.evaluate_prog_with_clock_def]
   \\ pairarg_tac \\ gvs []
   \\ qexists_tac ‘k’ \\ fs []
 QED
+
+
+Definition safe_dec'_def:
+  safe_dec' (Dlet locs pat x) = safe_exp x ∧
+  safe_dec' (Dletrec locs' funs) = EVERY safe_exp (MAP (SND ∘ SND) funs) ∧
+  safe_dec' _ = T
+End
+
+Theorem safe_dec_thm[local]:
+  safe_dec = every_dec safe_dec'
+Proof
+  fs [candle_prover_invTheory.safe_dec_def]
+  \\ AP_TERM_TAC
+  \\ fs [FUN_EQ_THM]
+  \\ Cases
+  \\ fs [safe_dec'_def]
+QED
+
+Definition safe_exp'_def:
+  (safe_exp' (Con (SOME i) _) = (id_to_n i ∉ kernel_ctors)) ∧
+  (safe_exp' (App (FFI n) _) = (n ≠ kernel_ffi)) ∧
+  (safe_exp' _ = T)
+End
+
+Theorem safe_exp_thm[local]:
+  safe_exp = every_exp safe_exp'
+Proof
+  fs [candle_prover_invTheory.safe_exp_def]
+  \\ AP_TERM_TAC
+  \\ fs [FUN_EQ_THM]
+  \\ Cases
+  \\ fs [safe_exp'_def]
+  >~ [‘safe_exp' (Con constructor args)’] >- (
+    Cases_on ‘constructor’ \\ fs [safe_exp'_def])
+  \\ rename1 ‘safe_exp' (App operator args)’
+  \\ Cases_on ‘operator’ \\ fs [safe_exp'_def]
+QED
+
+Theorem MAP_SND[local]:
+  MAP SND [] = [] ∧
+  MAP SND ((x1,x2)::xs) = x2 :: MAP SND xs
+Proof
+  fs []
+QED
+
+Theorem MAP_SND_SND[local]:
+  MAP (SND ∘ SND) [] = [] ∧
+  MAP (SND ∘ SND) ((x1,x2,x3)::xs) = x3 :: MAP (SND ∘ SND) xs
+Proof
+  fs []
+QED
+
+val _ = (max_print_depth := 12);
+
+local
+  fun cross [] xs = []
+    | cross (y::ys) xs = map (fn x => (y,x)) xs @ cross ys xs;
+  val cs = List.tabulate (256,fn n => stringSyntax.mk_chr (numSyntax.term_of_int n))
+in
+  val char_eq_lemmas = cross cs cs |> map mk_eq |> map EVAL;
+end
+
+val candle_suffix = let
+  val (prog,ty) = listSyntax.dest_list (rhs (concl compiler64_arm8_prog_def))
+  val (kernel,_) = listSyntax.dest_list
+    (rhs (concl candle_kernelProgTheory.candle_code_def))
+  in listSyntax.mk_list (List.drop (prog,length kernel),ty) end;
+
+Definition compiler64_arm8_candle_suffix_def:
+  compiler64_arm8_candle_suffix = ^candle_suffix
+End
+
+Theorem compiler64_arm8_kernel_prefix[local]:
+  compiler64_arm8_prog = candle_code ++ compiler64_arm8_candle_suffix
+Proof
+  rewrite_tac [compiler64_arm8_candle_suffix_def,compiler64_arm8_prog_def,
+               candle_kernelProgTheory.candle_code_def,
+               APPEND,locationTheory.unknown_loc_def,MAP]
+QED
+
+Theorem compiler64_arm8_suffix_safe[local]:
+  EVERY safe_dec compiler64_arm8_candle_suffix
+Proof
+  rewrite_tac [compiler64_arm8_candle_suffix_def,
+               APPEND,locationTheory.unknown_loc_def,EVERY_DEF]
+  \\ rpt conj_tac
+  \\ rewrite_tac [safe_dec_thm,EVERY_DEF,safe_dec'_def,MAP_SND_SND,
+                  safe_exp_thm,safe_exp'_def,MAP_SND,namespaceTheory.id_to_n_def,
+                  ast_extrasTheory.every_exp_def |> CONV_RULE (DEPTH_CONV ETA_CONV),
+                  ast_extrasTheory.every_dec_def |> CONV_RULE (DEPTH_CONV ETA_CONV)]
+  \\ rewrite_tac [EVAL “«[]» ∉ kernel_ctors”, EVAL “«::» ∉ kernel_ctors”]
+  \\ rewrite_tac
+       ([EVAL “kernel_ctors”,mlstringTheory.mlstring_11,CONS_11,NOT_CONS_NIL,NOT_NIL_CONS,
+         IN_INSERT,NOT_IN_EMPTY,EVAL “kernel_ffi”] @ char_eq_lemmas)
+  \\ EVAL_TAC
+QED
+
+Theorem compiler64_arm8_prog_eq_candle_code_append:
+  ∃prog. compiler64_arm8_prog = candle_code ++ prog ∧ EVERY safe_dec prog
+Proof
+  qexists_tac ‘compiler64_arm8_candle_suffix’
+  \\ rewrite_tac [compiler64_arm8_kernel_prefix,compiler64_arm8_suffix_safe]
+QED
+
+val _ = check_thm repl_prog_isPREFIX;
+val _ = check_thm evaluate_decs_compiler64_arm8_prog;
+val _ = check_thm semantics_prog_compiler64_arm8_prog;
+val _ = check_thm compiler64_arm8_prog_eq_candle_code_append;
