compiler/bootstrap/translation/compiler64Arm8ProgScript.sml
@@ -1,7 +1,7 @@
 (*
-  Native x64 entry point for the 64-bit compiler.
+  Native ARM8 entry point for the 64-bit compiler.
 *)
-Theory compiler64Prog[no_sig_docs]
+Theory compiler64Arm8Prog[no_sig_docs]
 Ancestors
   compiler64MainProg basis_ffi[qualified]
 Libs
@@ -15,7 +15,7 @@ val _ = temp_delsimps ["NORMEQ_CONV", "lift_disj_eq", "lift_imp_disj"];
 val _ = translation_extends "compiler64MainProg";
 
 Quote add_cakeml:
-  fun main u = main_host (Hostx64,u)
+  fun main u = main_host (Hostarm8,u)
 End
 
 val main_v_def = fetch "-" "main_v_def";
@@ -25,13 +25,12 @@ Theorem main_spec:
   app (p:'ffi ffi_proj) main_v [Conv NONE []]
       (STDIO fs * COMMANDLINE cl)
       (POSTv uv. &UNIT_TYPE () uv *
-       STDIO (full_compile_64 (TL cl) (get_stdin fs) fs) *
+       STDIO (full_compile_host HostArm8 (TL cl) (get_stdin fs) fs) *
        COMMANDLINE cl)
 Proof
   strip_tac
-  \\ once_rewrite_tac [GSYM full_compile_host_x64]
   \\ xcf_with_def main_v_def
-  \\ xlet `POSTv v. &COMPILER64HOST_COMPILER64_HOST_TYPE HostX64 v *
+  \\ xlet `POSTv v. &COMPILER64HOST_COMPILER64_HOST_TYPE HostArm8 v *
                 (STDIO fs * COMMANDLINE cl)`
   >- (
     simp [cfTheory.cf_con_def,semanticPrimitivesTheory.do_con_check_def,
@@ -50,14 +49,13 @@ QED
 Theorem main_whole_prog_spec:
   ~has_repl_flag (TL cl) /\ IS_SOME (stdin_content fs) ==>
   whole_prog_spec main_v cl fs NONE
-    ((=) (full_compile_64 (TL cl) (get_stdin fs) fs))
+    ((=) (full_compile_host HostArm8 (TL cl) (get_stdin fs) fs))
 Proof
   strip_tac
   \\ simp [basis_ffiTheory.whole_prog_spec_def]
-  \\ qexists_tac `full_compile_64 (TL cl) (get_stdin fs) fs`
+  \\ qexists_tac `full_compile_host HostArm8 (TL cl) (get_stdin fs) fs`
   \\ reverse conj_tac
-  >- simp [GSYM full_compile_host_x64,
-           GSYM full_compile_host_with_numchars,with_same_numchars]
+  >- simp [GSYM full_compile_host_with_numchars,with_same_numchars]
   \\ simp [SEP_CLAUSES]
   \\ irule (DISCH_ALL (MATCH_MP app_wgframe (UNDISCH main_spec)))
   \\ simp []
@@ -77,10 +75,10 @@ Proof
       parserProgTheory.peg_uqconstructorname_side_def]
 QED
 
-val sem_thm = prove_sem_thm "main" "compiler64_prog" main_whole_prog_spec;
-val compiler64_prog_def = fetch "-" "compiler64_prog_def";
+val sem_thm = prove_sem_thm "main" "compiler64_arm8_prog" main_whole_prog_spec;
+val compiler64_arm8_prog_def = fetch "-" "compiler64_arm8_prog_def";
 
-Theorem semantics_compiler64_prog:
+Theorem semantics_compiler64_arm8_prog:
   ~has_repl_flag (TL cl) /\ IS_SOME (stdin_content fs) /\ wfcl cl /\ wfFS fs /\
   STD_streams fs ==>
   ?io_events.
@@ -88,9 +86,9 @@ Theorem semantics_compiler64_prog:
       (init_state (basis_ffi ext cl fs) with
        eval_state := SOME (EvalDecs
          (eval_state_var with env_id_counter := (0,0,1))))
-      init_env compiler64_prog (Terminate Success io_events) /\
+      init_env compiler64_arm8_prog (Terminate Success io_events) /\
     extract_fs ext (cl,fs) io_events =
-      SOME (full_compile_64 (TL cl) (get_stdin fs) fs)
+      SOME (full_compile_host HostArm8 (TL cl) (get_stdin fs) fs)
 Proof
   strip_tac
   \\ irule sem_thm
@@ -102,35 +100,35 @@ val main_decls_thm = get_ml_prog_state ()
   |> ml_progLib.get_thm
   |> REWRITE_RULE [ml_progTheory.ML_code_def];
 
-Theorem BUTLAST_compiler64_prog[local]:
+Theorem BUTLAST_compiler64_arm8_prog[local]:
   ^(mk_eq (concl main_decls_thm |> rator |> rator |> rand,
-           ``BUTLAST compiler64_prog``))
+           ``BUTLAST compiler64_arm8_prog``))
 Proof
-  CONV_TAC (RAND_CONV (ONCE_REWRITE_CONV [compiler64_prog_def]))
+  CONV_TAC (RAND_CONV (ONCE_REWRITE_CONV [compiler64_arm8_prog_def]))
   \\ CONV_TAC (RAND_CONV (PURE_REWRITE_CONV [listTheory.FRONT_CONS]))
   \\ rewrite_tac []
 QED
 
-Theorem Decls_FRONT_compiler64_prog =
+Theorem Decls_FRONT_compiler64_arm8_prog =
   main_decls_thm
-  |> CONV_RULE (PATH_CONV "llr" (REWR_CONV BUTLAST_compiler64_prog))
+  |> CONV_RULE (PATH_CONV "llr" (REWR_CONV BUTLAST_compiler64_arm8_prog))
   |> CONV_RULE (RAND_CONV
        (EVAL THENC REWRITE_CONV (DB.find "_refs_def" |> map (#1 o #2)) THENC
         SIMP_CONV std_ss [APPEND_NIL,APPEND]))
   |> DISCH_ALL |> REWRITE_RULE [dec_sides];
 
-Theorem LAST_compiler64_prog:
-  LAST compiler64_prog =
+Theorem LAST_compiler64_arm8_prog:
+  LAST compiler64_arm8_prog =
     Dlet unknown_loc (Pcon NONE [])
       (App Opapp [Var (Short «main»); Con NONE []])
 Proof
   CONV_TAC (LAND_CONV
-    (ONCE_REWRITE_CONV [compiler64_prog_def] THENC
+    (ONCE_REWRITE_CONV [compiler64_arm8_prog_def] THENC
      PURE_REWRITE_CONV [listTheory.LAST_CONS]))
   \\ REFL_TAC
 QED
 
-val _ = semantics_compiler64_prog |> check_thm;
-val _ = Decls_FRONT_compiler64_prog |> check_thm;
-val _ = LAST_compiler64_prog |> check_thm;
+val _ = semantics_compiler64_arm8_prog |> check_thm;
+val _ = Decls_FRONT_compiler64_arm8_prog |> check_thm;
+val _ = LAST_compiler64_arm8_prog |> check_thm;
 val _ = ml_translatorLib.reset_translation ();
