compiler/bootstrap/translation/compiler64MainProgScript.sml
@@ -1,0 +1,421 @@
+(*
+  Shared entry points for the native 64-bit compiler programs.
+*)
+Theory compiler64MainProg[no_sig_docs]
+Ancestors
+  compiler64CommonProg compiler64Host compiler export ml_translator
+  basis_ffi[qualified]
+Libs
+  preamble ml_translatorLib cfLib basis
+
+open preamble compiler64CommonProgTheory compiler64HostTheory compilerTheory
+     exportTheory ml_translatorLib ml_translatorTheory
+open cfLib basis
+
+val _ = temp_delsimps ["NORMEQ_CONV", "lift_disj_eq", "lift_imp_disj"];
+val _ = translation_extends "compiler64CommonProg";
+val _ = ml_translatorLib.use_sub_check true;
+val _ = use_long_names := true;
+
+val spec64 = INST_TYPE [alpha |-> ``:64``];
+
+val _ = register_type ``:compiler64_host``;
+val _ = next_ml_names := ["host_args"];
+val r = translate host_args_def;
+
+Definition compiler_for_eval_def:
+  compiler_for_eval host = compile_inc_progs_for_eval (host_config host)
+End
+
+Theorem upper_w2w_eq_I[local]:
+  backend_common$upper_w2w = (I:word64 -> word64)
+Proof
+  fs [backend_commonTheory.upper_w2w_def,FUN_EQ_THM]
+QED
+
+val compiler_for_eval_alt =
+  [``HostX64``, ``HostArm8``]
+  |> map (fn host =>
+       ``compiler_for_eval ^host (id,c,ds)``
+       |> SIMP_CONV std_ss
+            [compiler_for_eval_def, host_config_def,
+             backendTheory.compile_inc_progs_for_eval_eq,
+             backendTheory.ensure_fp_conf_ok_def,
+             EVAL ``x64_config.reg_count``, EVAL ``arm8_config.reg_count``,
+             EVAL ``LENGTH x64_config.avoid_regs``,
+             EVAL ``LENGTH arm8_config.avoid_regs``,
+             EVAL ``x64_config.fp_reg_count``, EVAL ``arm8_config.fp_reg_count``,
+             EVAL ``x64_config.two_reg_arith``, EVAL ``arm8_config.two_reg_arith``,
+             EVAL ``x64_config.addr_offset``, EVAL ``arm8_config.addr_offset``,
+             EVAL ``x64_config.ISA``, EVAL ``arm8_config.ISA``,
+             EVAL ``x86_64 = ARMv7``, EVAL ``ARMv8 = ARMv7``,
+             listTheory.MAP_ID, upper_w2w_eq_I])
+  |> LIST_CONJ;
+
+val r = translate (word_to_wordTheory.compile_single_def |> spec64);
+val r = translate (word_to_wordTheory.full_compile_single_def |> spec64);
+val r = translate (word_to_wordTheory.full_compile_single_for_eval_def |> spec64);
+
+Theorem ws_to_chars_eq[local]:
+  ws_to_chars [] = [] /\
+  ws_to_chars (w::ws) = CHR (w2n w) :: ws_to_chars ws
+Proof
+  fs [semanticPrimitivesTheory.ws_to_chars_def]
+QED
+
+val r = translate ws_to_chars_eq;
+
+Theorem semanticprimitives_ws_to_chars_side[local]:
+  !ws. semanticprimitives_ws_to_chars_side ws
+Proof
+  `!w:word8. w2n w < 256` by (
+    strip_tac
+    >> assume_tac (w2n_lt |> INST_TYPE [alpha |-> ``:8``])
+    >> `dimword (:8) = 256` by EVAL_TAC
+    >> fs [])
+  >> Induct
+  >> simp [Once (fetch "-" "semanticprimitives_ws_to_chars_side_def")]
+QED
+
+val _ = update_precondition semanticprimitives_ws_to_chars_side;
+val _ = next_ml_names := ["compiler_for_eval"];
+val r = translate compiler_for_eval_alt;
+
+val _ = append_prog
+  ``[Dlet (Locs (POSN 1 2) (POSN 2 21)) (Pvar «eval_prim»)
+      (Fun «x» (Mat (Var (Short «x»))
+        [(Pcon NONE [Pvar «env»; Pvar «s1»; Pvar «decs»;
+                     Pvar «s2»; Pvar «bs»; Pvar «ws»],
+          App Eval [Var (Short «env»); Var (Short «s1»); Var (Short «decs»);
+                    Var (Short «s2»); Var (Short «bs»); Var (Short «ws»)])]))]``;
+
+Datatype:
+  eval_res = Compile_error 'a | Eval_result 'b 'c | Eval_exn 'd 'e
+End
+
+val _ = register_type ``:('a,'b,'c,'d,'e) eval_res``;
+
+Quote add_cakeml:
+  fun eval (host, ((s1,next_gen), (env,id), decs)) =
+    case compiler_for_eval host ((id,0),(s1,decs)) of
+      None => Compile_error "ERROR: failed to compile input\n"
+    | Some (s2,(bs,ws)) =>
+        let
+          val new_env = eval_prim (env,s1,decs,s2,bs,ws)
+        in Eval_result (new_env,next_gen) (s2,next_gen+1) end
+        handle e => Eval_exn e (s2,next_gen+1)
+End
+
+Quote exn_msg_dec = cakeml:
+  val _ = (TextIO.print (!Repl.errorMessage);
+           print_pp (pp_exn (!Repl.exn));
+           print "\n")
+End
+
+Definition report_exn_dec_def:
+  report_exn_dec = ^exn_msg_dec
+End
+
+val _ = next_ml_names := ["report_exn_dec"];
+val r = translate report_exn_dec_def;
+
+Quote add_cakeml:
+  fun report_exn e =
+  (Repl.exn := e;
+   Repl.errorMessage := "EXCEPTION: ";
+   report_exn_dec)
+End
+
+Quote error_msg_dec = cakeml:
+  val _ = TextIO.print (!Repl.errorMessage)
+End
+
+Definition report_error_dec_def:
+  report_error_dec = ^error_msg_dec
+End
+
+val _ = next_ml_names := ["report_error_dec"];
+val r = translate report_error_dec_def;
+
+Quote add_cakeml:
+  fun report_error msg =
+  (Repl.errorMessage := msg;
+   report_error_dec)
+End
+
+val _ = next_ml_names := ["roll_back"];
+val r = translate repl_check_and_tweakTheory.roll_back_def;
+val _ = next_ml_names := ["check_and_tweak"];
+val r = translate repl_check_and_tweakTheory.check_and_tweak_def;
+
+Quote add_cakeml:
+  fun repl (host, parse, types, conf, env, decs, input_str) =
+  case check_and_tweak (decs, (types, input_str)) of
+    Inl msg => repl (host, parse, types, conf, env, report_error msg, "")
+  | Inr (safe_decs, new_types) =>
+      case eval (host, (conf, env, safe_decs)) of
+        Compile_error msg =>
+          repl (host, parse, types, conf, env, report_error msg, "")
+      | Eval_exn e new_conf =>
+          repl (host, parse, roll_back (types, new_types), new_conf, env,
+                report_exn e, "")
+      | Eval_result new_env new_conf =>
+          if !Repl.isEOF then () else
+            let val new_input = !Repl.nextString in
+              case parse new_input of
+                Inl msg =>
+                  repl (host, parse, new_types, new_conf, new_env,
+                        report_error msg, "")
+              | Inr new_decs =>
+                  repl (host, parse, new_types, new_conf, new_env,
+                        new_decs, new_input)
+            end
+End
+
+val _ = next_ml_names := ["init_types"];
+val r = translate repl_init_typesTheory.repl_init_types_eq;
+
+Definition parse_cakeml_syntax_def:
+  parse_cakeml_syntax input =
+  case parse_prog (lexer_fun (explode input)) of
+  | Success _ x _ => INR x
+  | Failure l _ => INL («Parsing failed at » ^ locs_to_string input (SOME l))
+End
+
+Definition parse_ocaml_syntax_def:
+  parse_ocaml_syntax input =
+  case caml_parser$run (explode input) of
+  | INR res => INR res
+  | INL (l,err) =>
+      INL (err ^ «\nParsing failed at » ^ locs_to_string input (SOME l))
+End
+
+Definition select_parse_def:
+  select_parse cl =
+  if MEMBER «--candle» cl then parse_ocaml_syntax else parse_cakeml_syntax
+End
+
+val r = translate parse_cakeml_syntax_def;
+val r = translate parse_ocaml_syntax_def;
+val _ = next_ml_names := ["select_parse"];
+val r = translate select_parse_def;
+
+Definition init_next_string_def:
+  init_next_string cl = if MEM «--candle» cl then «candle» else «»
+End
+
+val _ = next_ml_names := ["init_next_string"];
+val r = translate (init_next_string_def |> REWRITE_RULE [MEMBER_INTRO]);
+
+Quote add_cakeml:
+  fun start_repl (host,cl,s1) =
+    let
+      val parse = select_parse cl
+      val types = init_types
+      val conf = (s1,1)
+      val env = (repl_init_env, 0)
+      val decs = []
+      val input_str = ""
+      val _ = Repl.nextString := init_next_string cl
+    in
+      repl (host, parse, types, conf, env, decs, input_str)
+    end
+End
+
+Quote add_cakeml:
+  fun run_interactive_repl (host,cl) =
+    let
+      val cs = Repl.charsFrom "config_enc_str.txt"
+      val s1 = decodeProg.decode_backend_config cs
+    in
+      start_repl (host,cl,s1)
+    end
+End
+
+Definition has_repl_flag_def:
+  has_repl_flag cl <=> MEM «--repl» cl \/ MEM «--candle» cl
+End
+
+val _ = next_ml_names := ["compiler_has_repl_flag"];
+val r = translate (has_repl_flag_def |> REWRITE_RULE [MEMBER_INTRO]);
+val r = translate (has_pancake_flag_def |> SIMP_RULE (srw_ss()) [MEMBER_INTRO]);
+
+Definition full_compile_host_def:
+  full_compile_host host cl inp fs =
+  if has_help_flag cl then
+    add_stdout fs help_string
+  else if has_version_flag cl then
+    add_stdout fs current_build_info_str
+  else
+    case parse_pancake_feature cl of
+      SOME rest => add_stdout fs $ print_bool $ news$query_news rest
+    | NONE =>
+        let (out, err) =
+            if has_pancake_flag cl then
+              compile_pancake_64 (host_args host cl) inp
+            else
+              compile_64 (host_args host cl) inp
+        in
+          add_stderr (add_stdout (fastForwardFD fs 0) (concat (append out))) err
+End
+
+Theorem full_compile_host_x64:
+  full_compile_host HostX64 cl inp fs = full_compile_64 cl inp fs
+Proof
+  simp [full_compile_host_def,full_compile_64_def]
+QED
+
+Quote add_cakeml:
+  fun main_host (host,u) =
+  let
+    val cl = CommandLine.arguments ()
+  in
+    if compiler_has_repl_flag cl then
+      run_interactive_repl (host,cl)
+    else if compiler_has_help_flag cl then
+      print compiler_help_string
+    else if compiler_has_version_flag cl then
+      print compiler_current_build_info_str
+    else
+      case compiler_parse_pancake_feature cl of
+        Some rest => print (compiler_print_bool (news_query_news rest))
+      | None =>
+          let val compile_cl = host_args host cl in
+            if compiler_has_pancake_flag cl then
+              case compiler_compile_pancake_64 compile_cl
+                     (String.explode (TextIO.inputAll (TextIO.openStdIn ()))) of
+                (c,e) => (print_app_list c; TextIO.output TextIO.stdErr e;
+                           compiler64commonprog_nonzero_exit_code_for_error_msg e)
+            else
+              case compiler_compile_64 compile_cl
+                     (String.explode (TextIO.inputAll (TextIO.openStdIn ()))) of
+                (c,e) => (print_app_list c; TextIO.output TextIO.stdErr e;
+                           compiler64commonprog_nonzero_exit_code_for_error_msg e)
+          end
+  end
+End
+
+val main_host_v_def = fetch "-" "main_host_v_def";
+
+Theorem main_host_spec:
+  COMPILER64HOST_COMPILER64_HOST_TYPE host host_v /\
+  ~has_repl_flag (TL cl) /\ IS_SOME (stdin_content fs) ==>
+  app (p:'ffi ffi_proj) main_host_v
+      [Conv NONE [host_v; Conv NONE []]] (STDIO fs * COMMANDLINE cl)
+      (POSTv uv.
+       &UNIT_TYPE () uv
+       * STDIO (full_compile_host host (TL cl) (get_stdin fs) fs)
+       * COMMANDLINE cl)
+Proof
+  rpt strip_tac
+  \\ xcf_with_def main_host_v_def
+  \\ xmatch
+  \\ xlet_auto >- (xcon \\ xsimpl)
+  \\ xlet_auto >- xsimpl
+  \\ reverse (Cases_on `STD_streams fs`)
+  >- (fs [STDIO_def] \\ xpull)
+  \\ reverse (Cases_on `?inp pos. stdin fs inp pos`)
+  >- (
+    fs [STDIO_def,IOFS_def] \\ xpull \\ fs [stdin_def]
+    \\ `F` suffices_by fs []
+    \\ fs [wfFS_def,STD_streams_def,MEM_MAP,Once EXISTS_PROD,PULL_EXISTS]
+    \\ fs [EXISTS_PROD]
+    \\ metis_tac [ALOOKUP_FAILS,ALOOKUP_MEM,NOT_SOME_NONE,SOME_11,
+                  PAIR_EQ,option_CASES])
+  \\ fs [get_stdin_def]
+  \\ SELECT_ELIM_TAC
+  \\ simp [FORALL_PROD,EXISTS_PROD]
+  \\ conj_tac >- metis_tac []
+  \\ rw []
+  \\ imp_res_tac stdin_11 \\ rw []
+  \\ imp_res_tac stdin_get_file_content
+  \\ xlet_auto >- xsimpl
+  \\ xif
+  \\ first_x_assum $ irule_at $ Pos hd \\ simp []
+  \\ xlet_auto >- xsimpl
+  \\ xif
+  >- (
+    simp [full_compile_host_def]
+    \\ xapp
+    \\ CONV_TAC SWAP_EXISTS_CONV
+    \\ qexists_tac `help_string`
+    \\ fs [compilerTheory.help_string_def,compiler_help_string_v_thm]
+    \\ xsimpl
+    \\ rename1 `add_stdout _ (strlit string)`
+    \\ CONV_TAC SWAP_EXISTS_CONV
+    \\ qexists_tac `fs`
+    \\ xsimpl)
+  \\ xlet_auto >- xsimpl
+  \\ xif
+  >- (
+    simp [full_compile_host_def]
+    \\ xapp
+    \\ CONV_TAC SWAP_EXISTS_CONV
+    \\ qexists_tac `current_build_info_str`
+    \\ fs [compilerTheory.current_build_info_str_def,
+           compiler_current_build_info_str_v_thm]
+    \\ xsimpl
+    \\ rename1 `add_stdout _ (strlit string)`
+    \\ CONV_TAC SWAP_EXISTS_CONV
+    \\ qexists_tac `fs`
+    \\ xsimpl)
+  \\ xlet_auto >- xsimpl
+  \\ gvs [oneline std_preludeTheory.OPTION_TYPE_def]
+  \\ reverse PURE_FULL_CASE_TAC
+  \\ gvs []
+  >- (
+    xmatch
+    \\ xlet_auto >- xsimpl
+    \\ xlet_auto >- xsimpl
+    \\ simp [full_compile_host_def]
+    \\ xapp
+    \\ first_assum $ irule_at $ Pos hd
+    \\ qexists_tac `fs`
+    \\ xsimpl)
+  \\ xmatch
+  \\ xlet_auto >- xsimpl
+  \\ xlet_auto >- xsimpl
+  \\ xif
+  \\ (
+    xlet_auto >- (xcon \\ xsimpl)
+    \\ rename [`stdin fs inp pos`]
+    \\ `stdin_content fs = SOME inp /\ pos = 0` by (
+      gvs [stdin_def,get_file_content_def]
+      \\ fs [stdin_content_def,IS_SOME_EXISTS])
+    \\ gvs []
+    \\ xlet_auto_spec (SOME openStdIn_spec_str) >- xsimpl
+    \\ xlet `POSTv v. &STRING_TYPE (implode inp) v *
+                    STDIO (fastForwardFD fs 0) * COMMANDLINE cl`
+    >- (
+      xapp
+      \\ qexistsl [`COMMANDLINE cl`, `inp`, `fs`, `0`]
+      \\ xsimpl)
+    \\ xlet_auto >- xsimpl
+    \\ xlet_auto >- xsimpl
+    \\ fs [full_compile_host_def]
+    \\ pairarg_tac
+    \\ fs [ml_translatorTheory.PAIR_TYPE_def]
+    \\ gvs [CaseEq "bool"]
+    \\ xmatch
+    \\ xlet_auto >- xsimpl
+    \\ qmatch_goalsub_abbrev_tac `STDIO output_fs`
+    \\ xlet `POSTv uv. &UNIT_TYPE () uv *
+                      STDIO (add_stderr output_fs err) * COMMANDLINE cl`
+    >- (
+      xapp_spec output_stderr_spec \\ xsimpl
+      \\ qexists_tac `COMMANDLINE cl`
+      \\ asm_exists_tac \\ xsimpl
+      \\ qexists_tac `output_fs` \\ xsimpl)
+    \\ xapp
+    \\ asm_exists_tac \\ simp [] \\ xsimpl)
+QED
+
+Theorem full_compile_host_with_numchars:
+  full_compile_host host cl inp (fs with numchars := ns) =
+  full_compile_host host cl inp fs with numchars := ns
+Proof
+  rw [full_compile_host_def,UNCURRY,fastForwardFD_with_numchars,
+      add_stdo_with_numchars]
+  \\ Cases_on `parse_pancake_feature cl`
+  \\ simp []
+QED
