compiler/bootstrap/compilation/sexpr32/README.md
@@ -1,0 +1,6 @@
+This directory generates the target-independent 32-bit compiler
+S-expression used by the x64 and ARM8 releases.
+
+[sexprBootstrap32Script.sml](sexprBootstrap32Script.sml):
+Produces an sexp print-out of the bootstrap translated compiler
+definition for the 32-bit version of the compiler.
